HOL-ETCS/Coproduct.thy
@@ -20,7 +20,7 @@ where
   left_coproj_cfunc_coprod: "f : X \<rightarrow> Z \<Longrightarrow> g : Y \<rightarrow> Z \<Longrightarrow> f\<amalg>g \<circ>\<^sub>c (left_coproj X Y)  = f" and
   right_coproj_cfunc_coprod: "f : X \<rightarrow> Z \<Longrightarrow> g : Y \<rightarrow> Z \<Longrightarrow> f\<amalg>g \<circ>\<^sub>c (right_coproj X Y)  = g" and
   cfunc_coprod_unique: "f : X \<rightarrow> Z \<Longrightarrow> g : Y \<rightarrow> Z \<Longrightarrow> h : X \<Coprod> Y \<rightarrow> Z \<Longrightarrow> 
-    h \<circ>\<^sub>c left_coproj X Y = f \<Longrightarrow> h \<circ>\<^sub>c right_coproj X Y = g \<Longrightarrow> h = f\<amalg>g"
+    h \<circ>\<^sub>c left_coproj X Y = f \<Longrightarrow> h \<circ>\<^sub>c right_coproj X Y = g \<Longrightarrow> h = f \<amalg> g"
 
 definition is_coprod :: "cset \<Rightarrow> cfunc \<Rightarrow> cfunc \<Rightarrow> cset \<Rightarrow> cset \<Rightarrow> bool" where
   "is_coprod W i\<^sub>0 i\<^sub>1 X Y \<longleftrightarrow> 
