HOL-ETCS/Monus.thy
@@ -1,0 +1,20 @@
+theory Monus
+  imports Add
+begin
+
+definition monus1 :: "cfunc" 
+  where "monus1 = (THE u. u : \<nat>\<^sub>c \<rightarrow> \<nat>\<^sub>c\<^bsup>\<nat>\<^sub>c\<^esup> \<and> u \<circ>\<^sub>c zero = ((left_coproj \<nat>\<^sub>c \<one>) \<circ>\<^sub>c (left_cart_proj \<nat>\<^sub>c \<one>))\<^sup>\<sharp> \<and> 
+  u \<circ>\<^sub>c successor = predecessor\<^bsup>\<nat>\<^sub>c\<^esup>\<^sub>f \<circ>\<^sub>c u)"
+
+
+
+
+definition monus2 :: "cfunc" 
+  where "monus2   = eval_func  \<nat>\<^sub>c \<nat>\<^sub>c \<circ>\<^sub>c (id \<nat>\<^sub>c \<times>\<^sub>f monus1)"
+
+
+definition monus :: "cfunc \<Rightarrow> cfunc \<Rightarrow> cfunc" (infixl "\<midarrow>\<^sub>\<nat>" 65)
+  where "m \<midarrow>\<^sub>\<nat> n = monus2 \<circ>\<^sub>c \<langle>m, n\<rangle>"
+
+
+end
